theories/Reflect.v
@@ -4,54 +4,59 @@ From LinearCore Require Import
 
 
 
-Variant Reflect (P : Prop) : bool -> Prop :=
+Variant Bool (P : Prop) : bool -> Prop :=
   | T (Y : P)
-      : Reflect P true
+      : Bool P true
   | F (N : ~P)
-      : Reflect P false
+      : Bool P false
   .
 
 
 
-Variant ReflectOpt {T} (P : T -> Prop) : option T -> Prop :=
+Variant Option {T} (P : T -> Prop) : option T -> Prop :=
   | S x (Y : P x)
-      : ReflectOpt P (Some x)
+      : Option P (Some x)
   | N (N : forall x, ~P x)
-      : ReflectOpt P None
+      : Option P None
   .
 
 
 
-Lemma iff P b (R : Reflect P b)
+Lemma bool_iff P b (R : Bool P b)
   : P <-> b = true.
 Proof. invert R; split; intro C; try tauto. discriminate C. Qed.
 
-Lemma niff P b (R : Reflect P b)
+Lemma bool_niff P b (R : Bool P b)
   : ~P <-> b = false.
 Proof. invert R; split; intro C; try tauto. discriminate C. Qed.
 
-Lemma det
-  P p (Rp : Reflect P p)
-  Q q (Rq : Reflect Q q)
+Lemma bool_eq
+  Q P (E : P <-> Q) b
+  : Bool P b <-> Bool Q b.
+Proof. split; intro R; (destruct R; constructor; [apply E; exact Y |]); intro C; apply N0; apply E; exact C. Qed.
+
+Lemma bool_det
+  P p (Rp : Bool P p)
+  Q q (Rq : Bool Q q)
   (E : P <-> Q)
   : p = q.
 Proof. invert Rp; invert Rq; tauto. Qed.
 
 Lemma and
-  P p (Rp : Reflect P p)
-  Q q (Rq : Reflect Q q)
-  : Reflect (P /\ Q) (p && q).
+  P p (Rp : Bool P p)
+  Q q (Rq : Bool Q q)
+  : Bool (P /\ Q) (p && q).
 Proof. invert Rp; invert Rq; constructor; tauto. Qed.
 
 Lemma or
-  P p (Rp : Reflect P p)
-  Q q (Rq : Reflect Q q)
-  : Reflect (P \/ Q) (p || q).
+  P p (Rp : Bool P p)
+  Q q (Rq : Bool Q q)
+  : Bool (P \/ Q) (p || q).
 Proof. invert Rp; invert Rq; constructor; tauto. Qed.
 
 
 
 Lemma opt_eq {T}
-  P Q (E : forall x : T, P x <-> Q x) opt
-  : ReflectOpt P opt <-> ReflectOpt Q opt.
+  Q P (E : forall x : T, P x <-> Q x) opt
+  : Option P opt <-> Option Q opt.
 Proof. split; intro R; (destruct R; constructor; [apply E; assumption |]); intros x C; eapply N0; apply E; exact C. Qed.
