theories/BoundIn.v
@@ -1,0 +1,98 @@
+From LinearCore Require
+  Map
+  Pattern
+  Reflect
+  Term
+  .
+From LinearCore Require Import
+  Invert
+  .
+
+
+
+Definition Reflect {T} (P : T -> Name.name -> Prop) (p : T -> Map.set) : Prop :=
+  forall t x, P t x <-> Map.In x (p t).
+Arguments Reflect {T} P p/.
+
+
+
+Definition Strict strict : Name.name -> Prop := Pattern.BoundIn (proj1_sig strict).
+  | SArg curried name
+      : Strict (Pattern.App curried name) name
+  | SRec curried name (bound_earlier : Strict curried name) argument
+      : Strict (Pattern.App curried argument) name
+  .
+
+Fixpoint strict s : Map.set :=
+  match s with
+  | Pattern.Ctr _ => Map.empty
+  | Pattern.App curried argument => Map.add argument tt (strict curried)
+  end.
+
+Lemma strict_spec : Reflect Strict strict. Proof.
+  split.
+  - intro S. induction S; cbn; apply Map.in_add; [left | right]. { reflexivity. } exact IHS.
+  - intro I. generalize dependent x. induction t; intros; cbn in *. { destruct I as [y M]. invert M. }
+    apply Map.in_add in I as [-> | I]; [left | right]. apply IHt. exact I.
+Qed.
+
+
+
+Variant Pattern : forall (pattern : Pattern.pattern) (name : Name.name), Prop :=
+  | PNam name
+      : Pattern (Pattern.Nam name) name
+  | PPat strict name (bound_in_strict : Strict strict name)
+      : Pattern (Pattern.Pat strict) name
+  .
+
+Definition pattern p : Map.set :=
+  match p with
+  | Pattern.Nam name => Map.singleton name tt
+  | Pattern.Pat s => strict s
+  end.
+
+Lemma pattern_spec : Reflect Pattern pattern. Proof.
+  split.
+  - intro S. invert S; cbn.
+    + apply Map.in_singleton. reflexivity.
+    + apply strict_spec. exact bound_in_strict.
+  - intro I. generalize dependent x. induction t; intros; cbn in *.
+    + apply Map.in_singleton in I as ->. constructor.
+    + constructor. apply strict_spec. exact I.
+Qed.
+
+
+
+(* Bound *anywhere* in a term: not only at the top-level (e.g. in a match) but also arbitrarily far from control flow. *)
+Inductive Term : forall (term : Term.term) (name : Name.name), Prop :=
+  | TMov name
+      : Term (Term.Mov name) name
+  | TRef name
+      : Term (Term.Ref name) name
+  | TApF function name (bound_in_function : Term function name) argument
+      : Term (Term.App function argument) name
+  | TApA argument name (bound_in_argument : Term argument name) function
+      : Term (Term.App function argument) name
+  | TFoV name type body
+      : Term (Term.For name type body) name
+  | TFoT type name (bound_in_type : Term type name) variable body
+      : Term (Term.For variable type body) name
+  | TFoB body name (bound_in_body : Term body name) variable type
+      : Term (Term.For variable type body) name
+  | TCaP pattern name (bound_in_pattern : Pattern pattern name) body_if_match other_cases
+      : Term (Term.Cas pattern body_if_match other_cases) name
+  | TCaB body_if_match name (bound_in_body : Term body_if_match name) pattern other_cases
+      : Term (Term.Cas pattern body_if_match other_cases) name
+  | TCaO other_cases name (bound_in_other_cases : Term other_cases name) pattern body_if_match
+      : Term (Term.Cas pattern body_if_match other_cases) name
+  .
+
+Fixpoint term t : Map.set :=
+  match t with
+  | Term.Mov name
+  | Term.Ref name => Map.singleton name tt
+  | Term.App function arg => Map.set_union (term function) (term arg)
+  | Term.For variable type body => Map.add variable tt (Map.set_union (term type) (term body))
+  | Term.Cas p body_if_match other_cases => Map.set_union (pattern p) (Map.set_union (term body_if_match) (term other_cases))
+  | _ => Map.empty
+  end.
