theories/Constructor.v
@@ -1,0 +1,39 @@
+From LinearCore Require
+  Name
+  Reflect
+  .
+From LinearCore Require Import
+  Invert
+  .
+
+Variant builtin : Set :=
+  .
+
+Definition builtin_eq (a b : builtin) := true.
+Arguments builtin_eq a b/.
+
+Lemma builtin_eq_spec a b
+  : Reflect.Bool (a = b) (builtin_eq a b).
+Proof. destruct a. Qed.
+
+
+
+Variant constructor : Set :=
+  | Builtin (builtin : builtin)
+  | UserDefined (name : Name.name)
+  .
+
+Definition eq (a b : constructor) :=
+  match a, b with
+  | Builtin a, Builtin b => builtin_eq a b
+  | UserDefined a, UserDefined b => Name.eqb a b
+  | _, _ => false
+  end.
+Arguments eq a b/.
+
+Lemma eq_spec a b
+  : Reflect.Bool (a = b) (eq a b).
+Proof.
+  destruct a as [a | a]; destruct b as [b | b]; try (constructor; tauto).
+  cbn. destruct (Name.spec a b); constructor. { subst. reflexivity. } intro C. apply N. invert C. reflexivity.
+Qed.
