theories/Match.v
@@ -1,0 +1,32 @@
+From LinearCore Require
+  Map
+  Pattern
+  Term
+  .
+From LinearCore Require Import
+  Invert
+  .
+
+
+
+Inductive Raw : forall (pattern : Pattern.raw) (term : Term.term) (matches : Map.to Term.term), Prop :=
+  | Ctr matches (E : Map.Empty matches) ctor
+      : Raw (Pattern.Ctr ctor) (Term.Ctr ctor) matches
+  | App
+      function_pattern function function_matches (function_matched : Raw function_pattern function function_matches)
+      argument_name (N : forall (I : Map.In function_matches argument_name), False)
+      (* can't match the same name twice in the same pattern ^^^ *)
+      argument matches (A : Map.Add argument_name argument function_matches matches)
+      : Raw (Pattern.App function_pattern argument_name) (Term.App function argument) matches
+  .
+
+Fixpoint raw pattern term :=
+  match pattern, term with
+  | Pattern.Ctr constructor_pattern, Term.Ctr constructor =>
+      if Constructor.eq constructor_pattern constructor then Some Map.empty else None
+  | Pattern.App function_pattern argument_name, Term.App function argument =>
+      match raw function_pattern function with None => None | Some function_matches =>
+        Map.checked_add Term.eq argument_name argument function_matches
+      end
+  | _, _ => None
+  end.
