theories/Pattern.v
@@ -1,0 +1,38 @@
+From LinearCore Require
+  Constructor
+  Name
+  .
+
+
+
+Inductive raw : Set :=
+  | Ctr (constructor : Constructor.constructor)
+  | App (curried : raw) (argument : Name.name)
+  .
+
+Inductive BoundIn : raw -> Name.name -> Prop :=
+  | SArg curried name
+      : BoundIn (App curried name) name
+  | SRec curried name (bound_earlier : BoundIn curried name) argument
+      : BoundIn (App curried argument) name
+  .
+Arguments BoundIn raw name.
+
+Inductive WellFormed : raw -> Prop :=
+  | WFCtr constructor
+      : WellFormed (Ctr constructor)
+  | WFApp curried argument (no_dup_name : forall (B : BoundIn curried argument), False)
+      : WellFormed (App curried argument)
+  .
+Arguments WellFormed raw.
+
+
+
+Definition strict : Type := { raw : raw | WellFormed raw }.
+
+
+
+Variant pattern : Type :=
+  | Nam (name : Name.name)
+  | Pat (strict : strict)
+  .
