theories/Term.v
@@ -1,0 +1,57 @@
+From LinearCore Require
+  Constructor
+  Name
+  Pattern
+  .
+From LinearCore Require Import
+  Invert
+  .
+
+
+
+Inductive term : Type :=
+  | Err
+  | Typ
+  | Prp
+  | Ctr (constructor : Constructor.constructor)
+  | Mov (name : Name.name)
+  | Ref (name : Name.name)
+  | App (function : term) (argument : term)
+  | For (variable : Name.name) (type : term) (body : term)
+  | Cas (pattern : Pattern.pattern) (body_if_match : term) (other_cases : term)
+  .
+
+Fixpoint eq a b :=
+  match a, b with
+  | Err, Err
+  | Typ, Typ
+  | Prp, Prp => true
+  | Ctr a, Ctr b => Constructor.eq a b
+  | Mov a, Mov b
+  | Ref a, Ref b => Name.eqb a b
+  | App fa aa, App fb ab => andb (eq fa fb) (eq aa ab)
+  | For va ta ba, For vb tb bb => andb (Name.eqb va vb) (andb (eq ta tb) (eq ba bb))
+  | Cas pa ba oa, For pb bb ob => andb (Pattern.eq pa pb) (andb (eq ba bb) (eq oa ob))
+  | _, _ => false
+  end.
+
+Lemma eq_spec a b
+  : Reflect.Bool (a = b) (eq a b).
+Proof.
+  generalize dependent b. induction a; destruct b;
+  try (constructor; intro D; discriminate D); try (constructor; reflexivity).
+  - unfold eq. destruct (Constructor.eq_spec constructor constructor0); constructor. { f_equal. assumption. }
+    intro E. apply N. invert E. reflexivity.
+  - simpl eq. destruct (Name.spec name name0); constructor. { f_equal. assumption. }
+    intro E. apply N. invert E. reflexivity.
+  - simpl eq. destruct (Name.spec name name0); constructor. { f_equal. assumption. }
+    intro E. apply N. invert E. reflexivity.
+  - simpl eq. destruct (IHa1 b1); cbn. 2: { constructor. intro E. apply N. invert E. reflexivity. }
+    subst. destruct (IHa2 b2); constructor. { f_equal. assumption. } intro E. apply N. invert E. reflexivity.
+  - simpl eq. destruct (Name.spec variable variable0); cbn in *. 2: { constructor. intro E. apply N. invert E. reflexivity. }
+    destruct (IHa1 b1); cbn. 2: { constructor. intro E. apply N. invert E. reflexivity. }
+    subst. destruct (IHa2 b2); constructor. { f_equal. assumption. } intro E. apply N. invert E. reflexivity.
+  - simpl eq. destruct (Name.spec variable variable0); cbn in *. 2: { constructor. intro E. apply N. invert E. reflexivity. }
+    destruct (IHa1 b1); cbn. 2: { constructor. intro E. apply N. invert E. reflexivity. }
+    subst. destruct (IHa2 b2); constructor. { f_equal. assumption. } intro E. apply N. invert E. reflexivity.
+Qed.
